src/itree/Opt2Sim.v
@@ -296,11 +296,11 @@ Section SIM.
                                  tgt_m)
         (SIM: forall up le1 sm tm,
             (<<MM1: match_mem mp sm tm>>) ->
-            gupaco4 (_sim_seq term) (cpn4 (_sim_seq term)) g up (to_deferred mp)
+            gupaco7 _sim_seq (cpn7 _sim_seq) g _ _ term up (to_deferred mp)
                     (@SeqState.mk (lang _) (` x : lunit <- denote_block le1 b_src;; (let (le2, _) := x in Ret (le2 ret_reg))) sm)
                     (@SeqState.mk (lang _) (` x : lunit <- denote_block le1 b_tgt;; (let (le2, _) := x in Ret (le2 ret_reg))) tm))
     :
-      gpaco4 (_sim_seq term) (cpn4 (_sim_seq term)) r g p (to_deferred (inst_gd i mp)) src tgt.
+      gpaco7 _sim_seq (cpn7 _sim_seq) r g _ _ term p (to_deferred (inst_gd i mp)) src tgt.
   Proof.
     clarify.
     dup MC. rename MC0 into UPDATE. eapply match_code2_opt_inv in UPDATE.
@@ -760,17 +760,17 @@ Section SIM.
                                tgt_m)
       (SIM: forall up le1 sm tm,
           (<<MM1: match_mem mp sm tm>>) ->
-          gupaco4 (_sim_seq term) (cpn4 (_sim_seq term)) g up (to_deferred mp)
+          gupaco7 _sim_seq (cpn7 _sim_seq) g _ _ term up (to_deferred mp)
                   (@SeqState.mk (lang _) (` x : lunit <- denote_block le1 b_src;; (let (le2, _) := x in Ret (le2 ret_reg))) sm)
                   (@SeqState.mk (lang _) (` x : lunit <- denote_block le1 b_tgt;; (let (le2, _) := x in Ret (le2 ret_reg))) tm))
     ,
-      gpaco4 (_sim_seq term) (cpn4 (_sim_seq term)) r g p (to_deferred (inst_gd i mp)) src tgt.
+      gpaco7 _sim_seq (cpn7 _sim_seq) r g _ _ term p (to_deferred (inst_gd i mp)) src tgt.
 
 
   Lemma sim_seq_tau_ub
         r g p d src tgt sm tm
     :
-      gpaco4 (_sim_seq term) (cpn4 (_sim_seq term)) r g p d
+      gpaco7 _sim_seq (cpn7 _sim_seq) r g _ _ term p d
              (@SeqState.mk (lang _) (tau;; trigger MemE.abort;; src) sm)
              (@SeqState.mk (lang _) tgt tm).
   Proof.
